CertiGC/spatial_graph_gc.v
@@ -25,33 +25,23 @@ Instance PointerValE_EqDec: EquivDec.EqDec (pointer_val * unit) eq.
   destruct u, u0. destruct (PV_eq_dec p p0); [left | right]; congruence.
 Defined.
 
-Instance SGBA_VST: SpatialGraphBasicAssum pointer_val (pointer_val * unit).
-  refine (Build_SpatialGraphBasicAssum pointer_val (pointer_val * unit) _ _).
+Instance SGBA_VST: PointwiseGraphBasicAssum pointer_val (pointer_val * unit).
+  refine (Build_PointwiseGraphBasicAssum pointer_val (pointer_val * unit) _ _).
 Defined.
 
 End pSGG_VST.
 
-Instance pSGG_VST: pSpatialGraph_GList.
-  refine (Build_pSpatialGraph_GList pointer_val NullPointer mpred SGBA_VST).
+Instance pSGG_VST: pPointwiseGraph_GList.
+  refine (Build_pPointwiseGraph_GList pointer_val NullPointer mpred SGBA_VST).
 Defined.
 
 (* Eval cbv in (reptype node_type). *)
 
-Definition vgamma2cdata (rpa : nat * addr) : reptype node_type :=
-  match rpa with
-  | (r, pa) => (pointer_val_val pa, (pointer_val_val pa, pointer_val_val pa))
-  end.
 
 Section sSGG_VST.
 
-  Definition binode (sh: share) (p: addr) (rpa: nat * addr): mpred :=
-    data_at sh node_type (vgamma2cdata rpa) (pointer_val_val p).
 
-  Instance SGP_VST (sh: share) : SpatialGraphPred addr (addr * unit) (nat * addr) unit pred.
-  refine (Build_SpatialGraphPred _ _ _ _ _ (binode sh) (fun _ _ => emp)).
-  Defined.
-
-  Instance MSLstandard sh : MapstoSepLog (AAV (SGP_VST sh)) (binode sh).
+Instance MSLstandard sh g nr p : MapstoSepLog (AAV (SGP_VST sh g)) (node_pred sh g p nr).
   Proof.
     intros. apply mkMapstoSepLog. intros.
     apply derives_precise with (memory_block sh (sizeof node_type) (pointer_val_val p)); [| apply memory_block_precise].
@@ -73,15 +63,15 @@ Section sSGG_VST.
       apply pointer_range_overlap_refl; auto; omega.
   Qed.
 
-Instance SGA_VST (sh: share) : SpatialGraphAssum (SGP_VST sh).
-  refine (Build_SpatialGraphAssum _ _ _ _ _ _ _ _ _ _ _).
+Instance SGA_VST (sh: share) : PointwiseGraphAssum (SGP_VST sh).
+  refine (Build_PointwiseGraphAssum _ _ _ _ _ _ _ _ _ _ _).
 Defined.
 
-Instance SGAvs_VST (sh: wshare): SpatialGraphAssum_vs (SGP_VST sh).
+Instance SGAvs_VST (sh: wshare): PointwiseGraphAssum_vs (SGP_VST sh).
   apply sepcon_unique_vertex_at; auto.
 Defined.
 
-Instance SGAvn_VST (sh: wshare): SpatialGraphAssum_vn (SGP_VST sh) NullPointer.
+Instance SGAvn_VST (sh: wshare): PointwiseGraphAssum_vn (SGP_VST sh) NullPointer.
   intros [? ?].
   simpl.
   unfold binode.
@@ -93,8 +83,8 @@ End sSGG_VST.
 
 Hint Extern 10 (@sepcon_unique2 _ _ _ _ _ (@vertex_at _ _ _ _ _ _)) => apply sepcon_unique_vertex_at; auto.
 
-Instance sSGG_VST (sh: wshare): @sSpatialGraph_GList pSGG_VST nat unit.
-  refine (Build_sSpatialGraph_GList pSGG_VST _ _ (SGP_VST sh) (SGA_VST sh) (SGAvs_VST sh) (SGAvn_VST sh)).
+Instance sSGG_VST (sh: wshare): @sPointwiseGraph_GList pSGG_VST nat unit.
+  refine (Build_sPointwiseGraph_GList pSGG_VST _ _ (SGP_VST sh) (SGA_VST sh) (SGAvs_VST sh) (SGAvn_VST sh)).
 Defined.
 
 Global Opaque pSGG_VST sSGG_VST.
